cleanups

HumanEvalLean/HumanEval123.lean
@@ -3,13 +3,10 @@ import Std
 open Std
 
 def collatzStep (n : Nat) : Nat :=
-  if n > 0 then
     if n % 2 = 0 then n / 2 else n * 3 + 1
-  else
-    1
 
 def CollatzRel : Nat → Nat → Prop := fun m n =>
-    n ≠ 1 ∧ collatzStep n = m
+    n > 1 ∧ collatzStep n = m
 
 instance : WellFoundedRelation { m : Nat // Acc CollatzRel m } := Acc.wfRel
 
@@ -34,7 +31,9 @@ theorem Std.compare_ne_eq [Ord α] [LawfulEqOrd α] {x y : α} :
     compare x y ≠ .eq ↔ x ≠ y := by
   simp
 
-instance : LawfulOrderOrd Nat := sorry
+instance : LawfulOrderOrd Nat where
+  isLE_compare := by grind [Nat.isLE_compare]
+  isGE_compare := by grind [Nat.isGE_compare]
 
 theorem oddCollatz_pairwise_distinct {n : Nat} {h : Acc CollatzRel n} :
     (oddCollatz n h).Pairwise (· ≠ ·) := by
@@ -44,9 +43,90 @@ theorem oddCollatz_pairwise_lt {n : Nat} {h : Acc CollatzRel n} :
     (oddCollatz n h).Pairwise (· < ·) := by
   simpa [oddCollatz, compare_eq_lt] using TreeSet.ordered_toList (α := Nat) (cmp := compare)
 
+theorem mod_two_eq_one_of_mem_oddCollatz {m n : Nat} {h : Acc CollatzRel n} (hm : m ∈ oddCollatz n h) :
+    m % 2 = 1 := by
+  simp only [oddCollatz, TreeSet.mem_toList] at hm
+  generalize (⟨n, h⟩ : Subtype _) = n at hm
+  generalize hg : (∅ : TreeSet Nat) = acc at hm
+  have hm' (k : Nat) : k ∈ acc → k % 2 = 1 := by simp [← hg]
+  clear hg
+  fun_induction oddCollatz.collectOddCollatz n acc <;> grind
+
+theorem collatzRel_collatzStep {n : Nat} (h : n > 1) :
+    CollatzRel (collatzStep n) n := by
+  grind [CollatzRel]
+
+theorem transGen_collatzRel_of_mem_oddCollatz {m n : Nat} {h : Acc CollatzRel n} (hm : m ∈ oddCollatz n h)
+    (hne : m ≠ n) :
+    Relation.TransGen CollatzRel m n := by
+  simp only [oddCollatz, TreeSet.mem_toList] at hm
+  generalize htmp : (⟨n, h⟩ : Subtype _) = s at hm
+  rw [show n = s.val by grind] at hne ⊢
+  clear htmp
+  generalize hg : (∅ : TreeSet Nat) = acc at hm
+  have hm' (k : Nat) : k ∈ acc → k ≠ s → Relation.TransGen CollatzRel k s := by simp [← hg]
+  clear hg
+  generalize htmp : s = n₀ at hm' hne ⊢
+  have hs : s = n₀ ∨ Relation.TransGen CollatzRel s n₀ := Or.inl htmp
+  clear htmp
+  fun_induction oddCollatz.collectOddCollatz s acc
+  · rename_i n' acc' h' ih
+    apply ih hm
+    · grind
+    · apply Or.inr
+      rcases hs with rfl | hs
+      · exact .single (collatzRel_collatzStep (by grind))
+      · refine .trans ?_ hs
+        exact .single (collatzRel_collatzStep (by grind))
+  · grind
+  · grind
+
+theorem mem_collectOddCollatz_of_mem {n : { n : Nat // Acc CollatzRel n }} {acc : TreeSet Nat}
+    {m : Nat} (h : m ∈ acc) :
+    m ∈ oddCollatz.collectOddCollatz n acc := by
+  fun_induction oddCollatz.collectOddCollatz n acc <;> grind
+
+theorem mem_self_collectOddCollatz {n : { n : Nat // Acc CollatzRel n }} {acc : TreeSet Nat}
+    (h : n.val % 2 = 1) :
+    n.val ∈ oddCollatz.collectOddCollatz n acc := by
+  fun_cases oddCollatz.collectOddCollatz n acc <;> grind [mem_collectOddCollatz_of_mem]
+
+attribute [grind =] TreeSet.mem_toList
+
+theorem mem_self_oddCollatz {n : Nat} {h : Acc CollatzRel n} (h' : n % 2 = 1) :
+    n ∈ oddCollatz n h := by
+  grind [oddCollatz, mem_self_collectOddCollatz]
+
+theorem collectOddCollatz_mono {n : { n : Nat // Acc CollatzRel n }} {acc' acc : TreeSet Nat}
+    (h : ∀ x, x ∈ acc' → x ∈ acc) {x : Nat} (hx : x ∈ oddCollatz.collectOddCollatz n acc') :
+    x ∈ oddCollatz.collectOddCollatz n acc := by
+  fun_induction oddCollatz.collectOddCollatz n acc generalizing acc' <;>
+    grind [oddCollatz.collectOddCollatz]
+
+theorem mem_oddCollatz_of_mem_oddCollatz_of_collatzRel {k m n : Nat} {hm hn}
+    (hmem : k ∈ oddCollatz m hm) (hrel : CollatzRel m n) :
+    k ∈ oddCollatz n hn := by
+  grind [oddCollatz, CollatzRel, oddCollatz.collectOddCollatz, collectOddCollatz_mono]
+
+theorem Acc.invTransGen {x y : α} (h₁ : Acc r x) (h₂ : Relation.TransGen r y x) : Acc r y := by
+  simpa [acc_transGen_iff] using h₁.transGen.inv h₂
+
+theorem mem_oddCollatz_of_mem_oddCollatz_of_transGen {k m n : Nat} {hn}
+    (hrel : Relation.TransGen CollatzRel m n) (hmem : k ∈ oddCollatz m (hn.invTransGen hrel)) :
+    k ∈ oddCollatz n hn := by
+  induction hrel
+  · grind [mem_oddCollatz_of_mem_oddCollatz_of_collatzRel]
+  · grind [Acc.inv, mem_oddCollatz_of_mem_oddCollatz_of_collatzRel]
+
+theorem mem_oddCollatz_of_transGen {m n : Nat} {hn : Acc CollatzRel n}
+    (h : Relation.TransGen CollatzRel m n) (h' : m % 2 = 1) :
+    m ∈ oddCollatz n hn := by
+  grind [mem_oddCollatz_of_mem_oddCollatz_of_transGen, mem_self_oddCollatz]
+
 theorem mem_oddCollatz_iff {m n : Nat} {h : Acc CollatzRel n} :
-    m ∈ oddCollatz n h ↔ m = n ∨ CollatzRel m n := by
-  sorry
+    m ∈ oddCollatz n h ↔ m % 2 = 1 ∧ (m = n ∨ Relation.TransGen CollatzRel m n) := by
+  grind [mod_two_eq_one_of_mem_oddCollatz, transGen_collatzRel_of_mem_oddCollatz,
+    mem_self_oddCollatz, mem_oddCollatz_of_transGen]
 
 /-!
 ## Prompt
